nondeterministic_dataflow/Loop.thy
@@ -7,6 +7,29 @@ imports
 begin
 
 
+fun choices_at where
+  "choices_at _ (Read p f) = csingle (Read p f)"
+| "choices_at _ (Write op p x) = csingle (Write op p x)"
+| "choices_at 0 (Choice ops) = cempty"
+| "choices_at (Suc n) (Choice ops) = cUnion (cimage (choices_at n) ops)"
+
+definition "choices op = cUnion (cimage (\<lambda>i. choices_at i op) natcUNIV)"
+
+abbreviation "sound_reads wire buf \<equiv> cfilter (\<lambda> op. case op of Read p f \<Rightarrow> p \<notin> ran wire \<or> buf p \<noteq> [] | _ \<Rightarrow> True)"
+
+corec loop_op :: "('op \<rightharpoonup> 'ip) \<Rightarrow> ('ip \<Rightarrow> 'd buf) \<Rightarrow>
+  ('ip, 'op, 'd) op \<Rightarrow> ('ip, 'op, 'd) op" where
+  "loop_op wire buf op = Choice (cimage (\<lambda> op. case op of
+     Read p f \<Rightarrow> (if p \<in> ran wire then loop_op wire (BTL p buf) (f (BHD p buf)) else Read p (\<lambda> x. loop_op wire buf (f x)))
+   | Write op' p x \<Rightarrow> (case wire p of None \<Rightarrow> Write (loop_op wire buf op') p x | Some q \<Rightarrow> loop_op wire (BENQ q x buf) op')  
+   ) (sound_reads wire buf (choices op)))"
+
+definition feedback_op ( "_ \<up>" [66] 65) where
+  "feedback_op op = map_op projr projr (loop_op (case_sum (Some o Inl) (\<lambda> _. None)) (\<lambda> _. []) op)"
+
+lemma
+  ""
+
 inductive loop_producing :: "('op \<rightharpoonup> 'ip) \<Rightarrow> ('ip \<Rightarrow> 'd buf) \<Rightarrow> ('ip, 'op, 'd) op \<Rightarrow> nat \<Rightarrow> bool" where
   "loop_producing wire buf end_op 0"
 | "p \<notin> ran wire \<Longrightarrow> loop_producing wire buf (Read p f) 0"
